simplifying match node

PikeEquiv.v
@@ -10,20 +10,20 @@ Require Import NFA PikeTree PikeVM.
 (* a tree and a thread are equivalent when they are about to execute the same thing *)
 (* this means when the tree represents a given regex and continuation, *)
 (* the thread is at a pc that will execute the nfa of that same regex and continuation *)
-Inductive tree_thread (code:code) (inp:input): (tree * group_map) -> LoopBool -> thread -> Prop :=
+Inductive tree_thread (code:code) (inp:input): (tree * group_map) -> thread -> Prop :=
 | tt_eq:
   forall tree gm pc b pc_cont pc_end r cont
     (TREE: bool_tree r cont inp b tree)
     (NFA: nfa_rep r code pc pc_cont)
     (CONT: continuation_rep cont code pc_cont pc_end),
-    tree_thread code inp (tree, gm) b (pc, gm, b).
+    tree_thread code inp (tree, gm) (pc, gm, b).
 
 (* the initial active thread and the initial active tree are related with the invariant *)
 Lemma initial_tree_thread:
   forall r code tree inp
     (COMPILE: compilation r = code)
     (TREE: bool_tree r [] inp CanExit tree),
-    tree_thread code inp (tree, empty_group_map) CanExit (0, empty_group_map, CanExit).
+    tree_thread code inp (tree, empty_group_map) (0, empty_group_map, CanExit).
 Proof.
   intros r code tree inp COMPILE TREE.
   unfold compilation in COMPILE. destruct (compile r 0) as [c fresh] eqn:COMP.
@@ -40,23 +40,26 @@ Inductive list_tree_thread (code:code) (inp:input) : list (tree * group_map) -> 
 | ltt_cons:
   forall treelist threadlist tree gm pc b
     (LTT: list_tree_thread code inp treelist threadlist)
-    (TT: tree_thread code inp (tree, gm) b (pc, gm, b)),
+    (TT: tree_thread code inp (tree, gm) (pc, gm, b)),
     list_tree_thread code inp ((tree,gm)::treelist) ((pc,gm,b)::threadlist).
 
-(* relating the best matches *)
-Inductive best_eq (inp:input) : option leaf -> option thread -> Prop :=
-| best_none: best_eq inp None None
-| best_some:
-  forall gm pc b, best_eq inp (Some (inp, gm)) (Some (pc, gm, b)).
+Lemma ltt_app:
+  forall code inp tl1 tl2 vl1 vl2
+    (LTT1: list_tree_thread code inp tl1 vl1)
+    (LTT2: list_tree_thread code inp tl2 vl2),
+    list_tree_thread code inp (tl1 ++ tl2) (vl1 ++ vl2).
+Proof.
+  intros. induction LTT1; auto. simpl. constructor; auto.
+Qed.
 
 (* lifting the equivalence predicate to pike states *)
 Inductive pike_inv (code:code): pike_tree_state -> pike_vm_state -> Prop :=
 | pikeinv:
-  forall inp idx treeactive treebest treeblocked threadactive threadbest threadblocked
+  forall inp idx treeactive treeblocked threadactive threadblocked best
     (ACTIVE: list_tree_thread code inp treeactive threadactive)
-    (BEST: best_eq inp treebest threadbest)
+    (* below is not correct: they must be equivalent for the next input *)
     (BLOCKED: list_tree_thread code inp treeblocked threadblocked),
-    pike_inv code (PTS idx treeactive treebest treeblocked) (PVS inp idx threadactive threadbest threadblocked).
+    pike_inv code (PTS idx treeactive best treeblocked) (PVS inp idx threadactive best threadblocked).
 
 (* the initial states of both smallstep semantics are related with the invariant *)
 Lemma initial_pike_inv:
@@ -74,3 +77,89 @@ Proof.
   - subst. apply nfa_rep_extend. auto.
   - constructor. replace (length c) with (length c + 0) by auto. rewrite get_prefix. auto.
 Qed.
+
+
+(** * Invariant Preservation  *)
+
+Theorem generate_active:
+  forall tree gm idx inp code pc b treeactive
+    (TREESTEP: tree_bfs_step tree gm idx = StepActive treeactive)
+    (TT: tree_thread code inp (tree, gm) (pc, gm, b)),
+  exists threadactive,
+    epsilon_step (pc, gm, b) code inp idx = EpsActive threadactive /\
+      list_tree_thread code inp treeactive threadactive.
+Proof.
+Admitted.
+
+Theorem generate_match:
+  forall tree gm idx inp code pc b
+    (TREESTEP: tree_bfs_step tree gm idx = StepMatch)
+    (TT: tree_thread code inp (tree, gm) (pc, gm, b)),
+    epsilon_step (pc, gm, b) code inp idx = EpsMatch.
+Proof.
+  intros tree gm idx inp code pc b TREESTEP TT.
+  unfold tree_bfs_step in TREESTEP. destruct tree; inversion TREESTEP. subst.
+  inversion TT. subst. inversion TREE; subst.
+  - unfold epsilon_step. inversion CONT. subst. inversion NFA. subst.
+    rewrite ACCEPT. auto.
+  (* issue: there are many ways to obtain a match tree. maybe it's epsilon, maybe epsilon;epsilon ... *)
+  (* these all have the same tree. not sure how to proceed for now *)
+  - admit.
+  - admit.
+  - admit.
+Admitted.
+
+(* TODO: there is too much info in EpsBlocked, StepMatch etc. Makes the theorem statements no very convenient *)
+Theorem generate_blocked:
+  forall tree gm idx inp code pc b nexttree
+    (TREESTEP: tree_bfs_step tree gm idx = StepBlocked nexttree)
+    (TT: tree_thread code inp (tree, gm) (pc, gm, b)),
+  exists nextthread,
+    epsilon_step (pc, gm, b) code inp idx = EpsBlocked nextthread /\
+      tree_thread code inp (nexttree,gm) nextthread.
+Proof.
+Admitted.
+
+
+Theorem invariant_preservation:
+  forall code pts1 pts2 pvs1
+    (INV: pike_inv code pts1 pvs1)
+    (TREESTEP: pike_tree_step pts1 pts2),
+  exists pvs2,
+    pike_vm_step code pvs1 pvs2 /\
+      pike_inv code pts2 pvs2.
+Proof.
+  intros. inversion INV. subst.
+  inversion TREESTEP; subst.
+  (* pts_nextchar *)
+  - inversion ACTIVE. subst.
+    (* the pike vm has two different rules for when we reach the end of input or not *)
+    destruct (advance_input inp) as [nextinp|] eqn:ADVANCE.
+    + exists (PVS nextinp (idx+1) threadblocked best []). split.
+      * apply pvs_nextchar. auto.
+      * constructor; auto.
+        ** admit.               (* we only have the eq for the previous input *)
+        ** admit.               (* same. ut for best, maybe we could only export the group_map *)
+    + exists (PVS inp idx [] best threadblocked). split.
+      * apply pvs_end. auto.
+      * admit.                  (* here there is an issue: the pike tree step loops but keeps increasing its index *)
+  (* pts_active *)
+  - inversion ACTIVE. subst. rename t into tree.
+    eapply generate_active in TT as [newthreads [EPS LTT2]]; eauto.
+    exists (PVS inp idx (newthreads++threadlist) best threadblocked). split.
+    + apply pvs_active. auto.
+    + apply pikeinv; auto. apply ltt_app; auto.
+  (* pts_match *)
+  - inversion ACTIVE. subst. rename t into tree.
+    eapply generate_match in TT; eauto.
+    exists (PVS inp idx [] (Some gm) threadblocked). split.
+    + apply pvs_match. auto.
+    + constructor; auto. constructor.
+  (* pts_blocked *)
+  - inversion ACTIVE. subst. rename t into tree.
+    eapply generate_blocked in TT as [nextt [EPS TT2]]; eauto.
+    exists (PVS inp idx threadlist best (threadblocked ++ [nextt])). split.
+    + apply pvs_blocked. auto.
+    + constructor; auto. apply ltt_app; auto.
+      inversion TT2. subst. constructor; auto. constructor.
+Admitted.
